Proofed skip_expr termination

poSTVM/poSTVM.thy
@@ -1,6 +1,6 @@
 theory poSTVM
   imports 
-    "~~/poST/poSTVM/poSTVM_state"
+    "~~/poST/poSTVM/poSTVM_state" 
 begin
 
 text "Type describing result of processing statement"
@@ -28,26 +28,147 @@ definition binary_op_exec :: "binary_op \<Rightarrow> basic_post_type \<Rightarr
     binary_op.Mul \<Rightarrow> basic_post_type_mul var1 var2| 
     binary_op.Div \<Rightarrow> basic_post_type_div var1 var2| 
     binary_op.Mod \<Rightarrow> basic_post_type_mod var1 var2)"
-
+(*
 text "Splitting stack to first part describing expression and other stack. Assuming stack starting with some expression operation"
-fun get_expr :: "stack  \<Rightarrow> stack * stack" where
-"get_expr []  = ([], [])" |
-"get_expr ((stack_op.Unary unary_op_option)#other)  = 
-  (let (expr_list,st) = (get_expr other) in ((stack_op.Unary unary_op_option) # expr_list,st))" |
-"get_expr ((stack_op.Binary binary_op)#other)  = 
-  (let (expr_list1,st1) = (get_expr other);
-       (expr_list2,st2) = (get_expr st1) in ((Binary binary_op) # expr_list1 @ expr_list2,st2))" |
-"get_expr ((stack_op.Value basic_post_type)#other)  = 
-  ([Value basic_post_type],other)" |
-"get_expr ((stack_op.Get var)#other)  = 
-  ([stack_op.Get var],other)" |
-"get_expr ((stack_op.GetArray var)#other)  = 
-  (let (expr_list1,st1) = (get_expr other) in ((stack_op.GetArray var) # expr_list1, st1))"|
-"get_expr ((stack_op.CheckProcStat v1 v2)#other)  = 
-  ([stack_op.CheckProcStat v1 v2],other)" |
-"get_expr ((stack_op.FunctionCall v1 v2)#other)  = 
-  ([stack_op.FunctionCall v1 v2],other)" |
-"get_expr lt  = ([],lt)"
+function (sequential) get_expr :: "stack  \<Rightarrow> stack * stack" where
+  "get_expr []  = ([], [])" |
+  "get_expr ((stack_op.Unary unary_op_option)#other)  = 
+    (let (expr_list,st) = (get_expr other) in ((stack_op.Unary unary_op_option) # expr_list,st))" |
+  "get_expr ((stack_op.Binary binary_op)#other)  = 
+    (let (expr_list1,st1) = (get_expr other);
+         (expr_list2,st2) = (get_expr st1);
+          new_st = ((Binary binary_op) # expr_list1) @ expr_list2 
+      in (new_st,st2))" |
+  "get_expr ((stack_op.Value basic_post_type)#other)  = 
+    ([Value basic_post_type],other)" |
+  "get_expr ((stack_op.Get var)#other)  = 
+    ([stack_op.Get var],other)" |
+  "get_expr ((stack_op.GetArray var)#other)  = 
+    (let (expr_list1,st1) = (get_expr other) in ((stack_op.GetArray var) # expr_list1, st1))"|
+  "get_expr ((stack_op.CheckProcStat v1 v2)#other)  = 
+    ([stack_op.CheckProcStat v1 v2],other)" |
+  "get_expr ((stack_op.FunctionCall v1 v2)#other)  = 
+    ([stack_op.FunctionCall v1 v2],other)" |
+  "get_expr other  = ([],other)"
+  by pat_completeness auto
+termination get_expr
+  apply (relation "measure (\<lambda>s. (size s))") 
+      apply auto
+  apply simp
+  done*)
+(*termination by size_change*)
+
+function inc :: "nat list \<Rightarrow> nat list" where
+"inc [] = []" |
+"inc (val#other) = (val + 1) # (inc other)"
+  by pat_completeness auto
+termination by lexicographic_order
+
+lemma "inc [] = []"
+  apply auto
+  done
+
+
+
+function (sequential) skip_expr :: "stack \<Rightarrow> stack" where 
+  "skip_expr [] = []"
+| "skip_expr ((stack_op.Unary _)#other)= skip_expr other"
+| "skip_expr ((stack_op.Binary _)#other)= skip_expr (skip_expr other)"
+| "skip_expr ((stack_op.Value _)#other) = other"
+| "skip_expr ((stack_op.Get _)#other) = other"
+| "skip_expr ((stack_op.GetArray _)#other) = skip_expr other"
+| "skip_expr ((stack_op.CheckProcStat _ _)#other) = other"
+| "skip_expr ((stack_op.FunctionCall _ _)#other) = other"
+| "skip_expr other = other"
+  by pat_completeness auto
+
+lemma length_skip_expr [termination_simp]:
+    "skip_expr_dom xs \<Longrightarrow> length (skip_expr xs) \<le> length xs"
+  by (induction xs rule: skip_expr.pinduct) (auto simp: skip_expr.psimps)
+
+termination skip_expr by lexicographic_order
+
+print_theorems
+
+lemma skip_expr_lessening:
+  "length (skip_expr xs) \<le> length xs"
+  by (induction xs rule: skip_expr.induct) auto
+
+lemma shift_skip_expr_lessening:
+  "length (skip_expr (skip_expr xs)) \<le> length (skip_expr xs)"
+  by (induction xs rule: skip_expr.induct) (auto simp add: skip_expr_lessening)
+
+lemma double_skip_expr_lessening : 
+    "length (skip_expr (skip_expr xs)) \<le> length xs"
+  by (induction xs rule: skip_expr.induct) (auto simp add: skip_expr_lessening  Nat.le_SucI)
+
+find_theorems " _ \<le> _ \<Longrightarrow> _ \<le> Suc _"
+
+
+(*TO DO*)
+function (sequential) get_one_expr :: "stack \<Rightarrow> stack" where
+  "get_one_expr [] = []"
+| "get_one_expr ((stack_op.Unary unary_op_option)#other) = (stack_op.Unary unary_op_option) # (get_one_expr other)"
+| "get_one_expr ((stack_op.Binary binary_op)#other) =
+  (let left = (get_one_expr other);
+       right = (get_one_expr (skip_expr other))
+    in (stack_op.Binary binary_op)#left@right)"
+| "get_one_expr ((stack_op.Value val)#other) = [stack_op.Value val]"
+| "get_one_expr ((stack_op.Get val)#other) = [stack_op.Get val]"
+| "get_one_expr ((stack_op.GetArray val)#other) = (stack_op.GetArray val)#(get_one_expr other)"
+| "get_one_expr ((stack_op.CheckProcStat val1 val2)#other) = [stack_op.CheckProcStat val1 val2]"
+| "get_one_expr ((stack_op.FunctionCall val1 val2)#other) = [stack_op.FunctionCall val1 val2]"
+| "get_one_expr other = []"
+  by pat_completeness auto
+
+print_theorems
+
+lemma const_get_one_expr [termination_simp]:
+      "get_one_expr_dom xs \<Longrightarrow> length ((get_one_expr xs) @ (skip_expr xs)) = length xs"
+  by (induction xs rule :get_one_expr.pinduct) (auto simp: get_one_expr.psimps)
+
+lemma const_l_get_one_expr [termination_simp]:
+      "get_one_expr_dom xs \<Longrightarrow> (length (get_one_expr xs)) + (length (skip_expr xs)) = length xs"
+  by (induction xs rule :get_one_expr.pinduct) (auto simp: get_one_expr.psimps)
+
+lemma const_l_buff_get_one_expr [termination_simp]:
+    "get_one_expr_dom xs \<Longrightarrow> (length (get_one_expr xs)) + (length (skip_expr xs)) = length xs"
+  apply (induct xs rule:get_one_expr.pinduct)
+                     apply (auto simp: get_one_expr.psimps)
+  done
+
+
+lemma skip_get_one_expr [termination_simp]:
+      "get_one_expr_dom xs \<Longrightarrow> length (get_one_expr xs) = (length xs) - length (skip_expr xs)"
+  apply (induct xs rule:get_one_expr.pinduct)
+                     apply (auto simp add: get_one_expr.psimps skip_expr_lessening Nat.Suc_diff_le)
+  done
+
+lemma length_get_one_expr [termination_simp]:
+    "get_one_expr_dom xs \<Longrightarrow> length (get_one_expr xs) \<le> (length xs)"
+  by (induction xs rule: get_one_expr.pinduct) (auto simp add: get_one_expr.psimps const_get_one_expr const_l_get_one_expr)
+
+termination get_one_expr by lexicographic_order
+
+(*TO DO get_expr as combination of get_simple_expr and skip_expr*)
+function (sequential) get_expr :: "stack \<Rightarrow> stack * stack" where
+"get_expr [] = ([],[])"
+| "get_expr ((stack_op.Unary unary_op_option)#other) = (let (res,rest) = get_expr other in ((stack_op.Unary unary_op_option)#res,rest))"
+| "get_expr ((stack_op.Binary binary_op)#other) =
+  (let (left,rest1)= (get_expr other);
+       (right,rest2) = (get_expr rest1)
+    in (((stack_op.Binary binary_op)#left@right),rest2))"
+| "get_expr ((stack_op.Value val)#other) = ([stack_op.Value val],other)"
+| "get_expr ((stack_op.Get val)#other) = ([stack_op.Get val],other)"
+| "get_expr ((stack_op.GetArray val)#other) = (let (res,rest) = get_expr other in ((stack_op.GetArray val)#res,rest))"
+| "get_expr ((stack_op.CheckProcStat val1 val2)#other) = ([stack_op.CheckProcStat val1 val2],other)"
+| "get_expr ((stack_op.FunctionCall val1 val2)#other) = ([stack_op.FunctionCall val1 val2],other)"
+| "get_expr other = ([],other)"
+  by pat_completeness auto
+
+lemma length_get_expr [termination_simp]:
+  "get_expr_dom xs \<Longrightarrow> (let (f,s) = get_expr xs in ((length s) \<le> length xs))"
+  by (induction xs rule: get_expr.pinduct) (auto simp add: get_expr.psimps)
 
 text "Unwind stack until end or break point returning stack starting with the following instruction"
 fun skip_after_break :: "stack \<Rightarrow> stack" where
@@ -153,25 +274,118 @@ fun exec_expr :: "stack \<Rightarrow> model_state \<Rightarrow> basic_post_type 
   None" |
 "exec_expr lt _ = None"
 
-(*TO DO*)
-text "Initialization of array"
-fun initialize_array :: "model_state \<Rightarrow> symbolic_var \<Rightarrow> model_state" where
-"initialize_array st var_name= st"
+definition get_ex :: "(string,nat) fmap" where
+"get_ex = fmap_of_list [(''a'',1::nat), (''b'',2::nat)]"
 
-(*TO DO*)
+definition self :: "(string,nat) fmap \<Rightarrow> (string,nat) fmap" where
+"self v = v"
+
+value "self (fmmap (\<lambda>x. x) get_ex)"
+
+text "Initialization of array"
+fun initialize_array :: "model_state \<Rightarrow> stacked_var_init \<Rightarrow> stacked_var_init" where
+"initialize_array st var= 
+  (case var of 
+    (stacked_var_init.Array interval values (Some expr_list)) \<Rightarrow> 
+      (stacked_var_init.Array
+        (case interval of
+          (stacked_array_interval.Expr exp1 exp2) \<Rightarrow> 
+            (stacked_array_interval.Int (basic_post_type_to_int (the (exec_expr exp1))) (basic_post_type_to_int (the (exec_expr exp2)))) |
+          (stacked_array_interval.Int int1 int2) =>
+            (stacked_array_interval.Int int1 int2))
+        (map 
+          (\<lambda>exp. (the (exec_expr exp)))
+          expr_list)
+        None) |
+    (stacked_var_init.Array interval values None) \<Rightarrow> 
+      (stacked_var_init.Array 
+        (case interval of
+          (stacked_array_interval.Expr exp1 exp2) \<Rightarrow> 
+            (stacked_array_interval.Int (basic_post_type_to_int (the (exec_expr exp1))) (basic_post_type_to_int (the (exec_expr exp2)))) |
+          (stacked_array_interval.Int int1 int2) =>
+            (stacked_array_interval.Int int1 int2)) 
+        values 
+        None))"
+
 text "Initialization of symbolic variable"
-fun initialize_symbolic :: "model_state \<Rightarrow> symbolic_var \<Rightarrow> model_state" where
-"initialize_symbolic st var_name= st"
+fun initialize_symbolic :: "model_state \<Rightarrow> stacked_var_init  \<Rightarrow> stacked_var_init" where
+"initialize_symbolic st var= 
+  (case var of
+    (stacked_var_init.Symbolic value (Some init_stack)) \<Rightarrow> 
+      (stacked_var_init.Symbolic (the (exec_expr init_stack st)) None) |
+    (stacked_var_init.Symbolic value None) \<Rightarrow> 
+      (stacked_var_init.Symbolic value None))"
+
+(*TO DO FunctionBlock init*)
+text "Initialization of stacked var"
+fun initialize_stacked_vars :: "model_state \<Rightarrow> stacked_vars \<Rightarrow> stacked_vars" where
+"initialize_stacked_vars st vars =
+  (fmmap
+    (\<lambda>init.
+      (case init of
+        (stacked_var_init.Symbolic value init_option) \<Rightarrow> (initialize_symbolic st init) |
+        (stacked_var_init.Array interval values init_option) \<Rightarrow> (initialize_array st init) |
+        (stacked_var_init.FunctionBlock name) \<Rightarrow> (stacked_var_init.FunctionBlock name)) )
+    vars) "
+
+text "Initialization of proc_vars"
+fun initialize_stacked_proc_vars :: "model_state \<Rightarrow> stacked_proc_var list \<Rightarrow> stacked_proc_var list" where
+"initialize_stacked_proc_vars _ [] = []" |
+"initialize_stacked_proc_vars st (proc_var#other) = 
+  ((case proc_var of
+    (stacked_proc_var.Var stacked_vars) \<Rightarrow> (stacked_proc_var.Var (initialize_stacked_vars stacked_vars))|
+    (stacked_proc_var.ProcessVar var) \<Rightarrow> (stacked_proc_var.ProcessVar var)|
+    (stacked_proc_var.InOutVar stacked_vars) \<Rightarrow> (stacked_proc_var.InOutVar (initialize_stacked_vars stacked_vars)) |
+    (stacked_proc_var.InVar stacked_vars) \<Rightarrow> (stacked_proc_var.InVar (initialize_stacked_vars stacked_vars))|
+    (stacked_proc_var.OutVar stacked_vars) \<Rightarrow> (stacked_proc_var.OutVar (initialize_stacked_vars stacked_vars)))
+  #(initialize_stacked_proc_vars st other))"
 
 (*TO DO*)
 text "Initialization of process variables"
 fun initialize_process_vars :: "model_state \<Rightarrow> model_state" where
-"initialize_process_vars st =st"
+"initialize_process_vars (model_state.ST global_vars_list (program_map,cur_prog_name) fb_decl_list f_decl_list) =
+  (let st = (model_state.ST global_vars_list (program_map,cur_prog_name) fb_decl_list f_decl_list) 
+  in  (model_state.ST 
+    global_vars_list 
+    (fmmap 
+       (\<lambda>(var_list,proc_map,proc_name). 
+          (var_list,
+            (fmmap 
+              (\<lambda>(var_list,v1,v2,v3,v4).
+                (initialize_stacked_proc_vars st var_list,v1,v2,v3,v4))
+              proc_map),
+          proc_name)) 
+       program_map,
+      cur_prog_name) 
+    fb_decl_list 
+    f_decl_list))"
+
+text "Initialization of prog_vars"
+fun initialize_stacked_prog_vars :: "model_state \<Rightarrow> stacked_prog_var list \<Rightarrow> stacked_prog_var list" where
+"initialize_stacked_prog_vars _ [] = []" |
+"initialize_stacked_prog_vars st (prog_var#other) = 
+  ((case prog_var of
+    (stacked_prog_var.ExtVar stacked_vars) \<Rightarrow> (stacked_prog_var.ExtVar (initialize_stacked_vars st stacked_vars))|
+    (stacked_prog_var.Var stacked_vars) \<Rightarrow> (stacked_prog_var.Var (initialize_stacked_vars st stacked_vars))|
+    (stacked_prog_var.InOutVar stacked_vars) \<Rightarrow> (stacked_prog_var.InOutVar (initialize_stacked_vars st stacked_vars))|
+    (stacked_prog_var.InVar stacked_vars) \<Rightarrow> (stacked_prog_var.InVar (initialize_stacked_vars st stacked_vars))|
+    (stacked_prog_var.OutVar stacked_vars) \<Rightarrow> (stacked_prog_var.OutVar (initialize_stacked_vars st stacked_vars)))
+   #(initialize_stacked_prog_vars st other))"
 
 (*TO DO*)
 text "Initialization of program variables"
 fun initialize_program_vars :: "model_state \<Rightarrow> model_state" where
-"initialize_program_vars st =st"
+"initialize_program_vars (model_state.ST global_vars_list (program_map,cur_prog_name) fb_decl_list f_decl_list) =
+  (let st = (model_state.ST global_vars_list (program_map,cur_prog_name) fb_decl_list f_decl_list)
+  in (model_state.ST 
+    global_vars_list 
+    (fmmap 
+       (\<lambda>(var_list,proc_map,proc_name). 
+          (initialize_stacked_prog_vars st var_list,proc_map,proc_name)) 
+       program_map,
+      cur_prog_name) 
+    fb_decl_list 
+    f_decl_list))"
 
 text "Executing first full statement from stack returning other stack part modified model state and result of statement. Assuming stack starting from some statement operation. Assuming all variables initialized."
 fun exec_statement :: "stack \<Rightarrow> model_state \<Rightarrow> stack * model_state * statement_result" and
